\documentclass{article}

\usepackage{amsmath}
\usepackage{amssymb}
\usepackage{etoolbox}

%\usepackage{MinionPro}
%\usepackage{MnSymbol}

%\let\dmath\equation\let\enddmath\endequation
\usepackage{breqn}

\usepackage{phfqit}
%\usepackage[llanglefrommnsymbolfonts=false]{phfqit}


\phfqitDefineNorm\opnorm{}{_\infty}

\begin{document}

\begin{align*}
  x &= \Re(z)\ ; & y &= \Im(z)\ .
\end{align*}

Kets \& bras!
\begin{gather*}
  \ket{x} + \ket`\Big{\psi_-^{(e^x)}} + \ket[\Big]{\psi_-^{(e^x)}} = \ket*{\sum_j A_j}
  \\
  \bra{x} + \bra`\Big{\psi_-^{(e^x)}} + \bra[\Big]{\psi_-^{(e^x)}} = \bra*{\sum_j A_j}
  \\
  \proj{x} + \proj`\Big{\psi_-^{(e^x)}} + \proj[\Big]{\psi_-^{(e^x)}} = \proj*{\sum_j A_j}
  \\
  \braket{x}{y} + \braket`\Big{G}{\psi_-^{(e^x)}} + \braket[\Big]{z}{\psi_-^{(e^x)}}
  = \braket*{X}{\sum_j A_j}
  \\
  \ketbra{x}{y} + \ketbra`\Big{G}{\psi_-^{(e^x)}} + \ketbra[\Big]{z}{\psi_-^{(e^x)}}
  = \ketbra*{X}{\sum_j A_j}
  \\
  \dmatrixel{x}{y} + \dmatrixel`\Big{\phi}{G_-^{(e^x)}} 
  + \dmatrixel[\Big]{\phi}{G_-^{(e^x)}}
  = \dmatrixel*{X}{\sum_j A_j}
  \\
  \innerprod{x}{y} + \innerprod`\Big{G}{\psi_-^{(e^x)}} + \innerprod[\Big]{z}{\psi_-^{(e^x)}}
  = \innerprod*{X}{\sum_j A_j}
  \\
  \matrixel{x}{y}{z} + \matrixel`\Big{\phi}{G_-^{(e^x)}}{z}
  + \matrixel[\Big]{\phi}{G_-^{(e^x)}}{z}
  = \matrixel*{X}{\sum_j A_j}{z}
\end{gather*}

Operator kets \& bras!
\begin{gather*}
 \oket{x} +\oket`\Big{\psi_-^{(e^x)}} +\oket[\Big]{\psi_-^{(e^x)}} =\oket*{\sum_j A_j}
  \\
 \obra{x} +\obra`\Big{\psi_-^{(e^x)}} +\obra[\Big]{\psi_-^{(e^x)}} =\obra*{\sum_j A_j}
  \\
 \oproj{x} +\oproj`\Big{\psi_-^{(e^x)}} +\oproj[\Big]{\psi_-^{(e^x)}} =\oproj*{\sum_j A_j}
  \\
 \obraket{x}{y} +\obraket`\Big{G}{\psi_-^{(e^x)}} +\obraket[\Big]{z}{\psi_-^{(e^x)}}
  =\obraket*{X}{\sum_j A_j}
  \\
 \oketbra{x}{y} +\oketbra`\Big{G}{\psi_-^{(e^x)}} +\oketbra[\Big]{z}{\psi_-^{(e^x)}}
  =\oketbra*{X}{\sum_j A_j}
  \\
 \odmatrixel{x}{y} +\odmatrixel`\Big{\phi}{G_-^{(e^x)}} 
  +\odmatrixel[\Big]{\phi}{G_-^{(e^x)}}
  =\odmatrixel*{X}{\sum_j A_j}
  \\
 \omatrixel{x}{y}{z} +\omatrixel`\Big{\phi}{G_-^{(e^x)}}{z}
  +\omatrixel[\Big]{\phi}{G_-^{(e^x)}}{z}
  =\omatrixel*{X}{\sum_j A_j}{z}
\end{gather*}


Norms \& delimited stuff;
\begin{gather*}
  \norm`\Big{\sum_j A} = \norm[\Big]{\sum_j A} \leqslant \norm{B} -
  \norm*{C_9^\dagger}\ ;
  \\
  \opnorm`\Big{\sum_j A} = \opnorm[\Big]{\sum_j A} \leqslant \opnorm{B} -
  \opnorm*{C_9^\dagger}\ ;
  \\
  \abs*{\sum_j A^\dagger} = \abs`*{\sum_j A^\dagger} = \abs[\Big]{A} =
  \abs`\Big{A}
\end{gather*}

\begin{align*}
  \Gamma &= \ee^{-\beta H}
\end{align*}

\renewcommand\phfqitExpPowerExpression[1]{\exp\left\{#1\right\}}
\begin{dmath}
  \Gamma = \ee^{-\beta H}
\end{dmath}


\end{document}
